src/Specific/IntegrationTestMontgomeryP256_128Display.v
@@ -1,4 +1,4 @@
 Require Import Crypto.Specific.IntegrationTestMontgomeryP256_128.
 Require Import Crypto.Specific.IntegrationTestDisplayCommon.
 
-Check display mulmod_256.
+Check display mul.
